Make the types of the finite map type classes more specific.
This makes type checking more directed, and somewhat more predictable.

On the downside, it makes it impossible to declare the singleton on
lists as an instance of SingletonM and the insert and alter operations
on functions as instances of Alter and Insert. However, these were not
used often anyway.

prelude/functions.v
@@ -2,10 +2,10 @@ From iris.prelude Require Export base tactics.
 
 Section definitions.
   Context {A T : Type} `{∀ a b : A, Decision (a = b)}.
-  Global Instance fn_insert : Insert A T (A → T) :=
-    λ a t f b, if decide (a = b) then t else f b.
-  Global Instance fn_alter : Alter A T (A → T) :=
-    λ (g : T → T) a f b, if decide (a = b) then g (f a) else f b.
+  Definition fn_insert (a : A) (t : T) (f : A → T) : A → T := λ b,
+    if decide (a = b) then t else f b.
+  Definition fn_alter (g : T → T) (a : A) (f : A → T) : A → T := λ b,
+    if decide (a = b) then g (f a) else f b.
 End definitions.
 
 (* TODO: For now, we only have the properties here that do not need a notion
@@ -14,17 +14,17 @@ End definitions.
 Section functions.
   Context {A T : Type} `{∀ a b : A, Decision (a = b)}.
 
-  Lemma fn_lookup_insert (f : A → T) a t : <[a:=t]>f a = t.
-  Proof. unfold insert, fn_insert. by destruct (decide (a = a)). Qed.
+  Lemma fn_lookup_insert (f : A → T) a t : fn_insert a t f a = t.
+  Proof. unfold fn_insert. by destruct (decide (a = a)). Qed.
   Lemma fn_lookup_insert_rev  (f : A → T) a t1 t2 :
-    <[a:=t1]>f a = t2 → t1 = t2.
+    fn_insert a t1 f a = t2 → t1 = t2.
   Proof. rewrite fn_lookup_insert. congruence. Qed.
-  Lemma fn_lookup_insert_ne (f : A → T) a b t : a ≠ b → <[a:=t]>f b = f b.
-  Proof. unfold insert, fn_insert. by destruct (decide (a = b)). Qed.
+  Lemma fn_lookup_insert_ne (f : A → T) a b t : a ≠ b → fn_insert a t f b = f b.
+  Proof. unfold fn_insert. by destruct (decide (a = b)). Qed.
 
-  Lemma fn_lookup_alter (g : T → T) (f : A → T) a : alter g a f a = g (f a).
-  Proof. unfold alter, fn_alter. by destruct (decide (a = a)). Qed.
+  Lemma fn_lookup_alter (g : T → T) (f : A → T) a : fn_alter g a f a = g (f a).
+  Proof. unfold fn_alter. by destruct (decide (a = a)). Qed.
   Lemma fn_lookup_alter_ne (g : T → T) (f : A → T) a b :
-    a ≠ b → alter g a f b = f b.
-  Proof. unfold alter, fn_alter. by destruct (decide (a = b)). Qed.
+    a ≠ b → fn_alter g a f b = f b.
+  Proof. unfold fn_alter. by destruct (decide (a = b)). Qed.
 End functions.
